Why Dafny, why.

circular-array.dfy
@@ -1,40 +1,117 @@
+/*
+  Class CircularArray.
+*/
 class {:autocontracts} CircularArray {
 
-  // Implementation.
+  /*
+    Implementation.
+  */
   var arr: array<int>;
-  var maxAmount: nat;
-  var tailIndex: nat;
+  var startIndex: nat;
+  var nextIndex: nat;
+  var elementsCount: nat;
 
-  // Abstraction.
+  /*
+    Abstraction.
+  */
   ghost var Content: seq<int>;
-  ghost var MaxAmount: nat;
 
-  // Class invariant.
+  /*
+    Class invariant.
+  */
   ghost predicate Valid()
-    {
-      maxAmount > 0 &&
-      arr.Length == maxAmount &&
-      0 <= tailIndex <= maxAmount &&
-      Content == arr[0..tailIndex] &&
-      MaxAmount == maxAmount
-    }
-
-  // Constructor.
-  constructor CircularArray(initialSize: int)
-    requires initialSize > 0;
-    ensures Valid();
-    ensures Content == [];
-    ensures MaxAmount == initialSize;
   {
-    arr := new int[initialSize];
-    tailIndex := 0;
-    maxAmount := initialSize;
-    MaxAmount := initialSize;
+    0 <= startIndex <= arr.Length &&
+    0 <= nextIndex <= arr.Length &&
+    elementsCount <= arr.Length &&
+    (startIndex <= nextIndex ==> Content == arr[startIndex..nextIndex]) &&
+    (startIndex > nextIndex ==> Content == arr[startIndex..arr.Length] + arr[0..nextIndex])
+  }
+
+  /*
+    Constructor.
+  */
+  constructor WithInitialCapacity(initialCapacity: nat)
+    requires initialCapacity > 0
+    ensures Valid()
+    ensures arr.Length == initialCapacity
+    ensures startIndex == 0
+    ensures nextIndex == 0
+    ensures elementsCount == 0
+    ensures Content == []
+  {
+    arr := new int[initialCapacity];
+    startIndex := 0;
+    nextIndex := 0;
+    elementsCount := 0;
     Content := [];
   }
+
+  /*
+    Methods.
+  */
+
+  /*
+    Enqueue
+  */
+  method Enqueue(element: int)
+    requires Valid()
+    ensures Valid()
+    ensures elementsCount == old(elementsCount) + 1
+  {
+    /*
+      If the next index is equal to the length of the array, then we need to
+      reset it to 0.
+    */
+    if (nextIndex == arr.Length)
+    {
+      nextIndex := 0;
+    }
+    /*
+      If the array is full, then we need to create a new array with double
+      the capacity of the current array.
+    */
+    if (elementsCount == arr.Length)
+    {
+      var newArr := new int[arr.Length * 2];
+      var i := 0;
+      var j := startIndex;
+      while (i < arr.Length)
+        invariant 0 <= i <= arr.Length <= newArr.Length
+        decreases arr.Length - i
+      {
+        newArr[i] := arr[j % arr.Length];
+        i := i + 1;
+        j := j + 1;
+      }
+      nextIndex := arr.Length;
+      startIndex := 0;
+      arr := newArr;
+    }
+    /*
+      Add the element to the array.
+    */
+    arr[nextIndex] := element;
+    /*
+      Update variables.
+    */
+    nextIndex := nextIndex + 1;
+    elementsCount := elementsCount + 1;
+    if (startIndex <= nextIndex)
+    {
+      Content := arr[startIndex..nextIndex];
+    } else
+    {
+      Content := arr[startIndex..arr.Length] + arr[0..nextIndex];
+    }
+  }
+
 }
 
 method Main()
 {
-  var a := [1,2,3][0..0];
+  var queue := new CircularArray.WithInitialCapacity(5);
+  queue.Enqueue(1);
+  queue.Enqueue(2);
+  print queue.arr;
 }
